\documentclass{article}
\usepackage{amsmath}
\newcommand{\FoxH}[5]{H_{#2}^{#1}\left(#3\:\middle\vert\: \begin{subarray}{l}#4\\[0.4em] #5\end{subarray}\right)}
\begin{document}
\begin{align*}
\FoxH{2,3}{2,1}{\cdot}{\left(1, \frac{1}{\alpha }\right), \left(\text{Ceil}(\beta ), \beta\right)}{\left(\frac{1}{2}, \frac{\alpha }{2}\right), \left(1, 1\right), \left(1, \frac{\alpha }{2}\right)}
\end{align*}
\noindent\textbf{Summary}
\begin{align*}
a^* &= \frac{1}{\alpha }-\beta +1 \\
\Delta &= \alpha -\frac{1}{\alpha }-\beta +1 \\
\delta &= 2^{-\alpha } \left(\frac{1}{\alpha }\right)^{-1/\alpha } \left(2^{\alpha /2} \alpha ^{\alpha /2}+\alpha ^{\alpha }\right) \beta ^{-\beta } \\
\mu &= 1-\text{Ceil}(\beta ) \\
a_1^* &= \frac{1}{2} (\alpha -2 \beta +2) \\
a_2^* &= \frac{1}{\alpha }-\frac{\alpha }{2} \\
\xi &= \frac{3}{2}-\text{Ceil}(\beta ) \\
c^* &= \frac{1}{2} \\
\end{align*}
\end{document}